square_bij.v
@@ -5,7 +5,7 @@ From Coq Require Import
     Utf8
 .
 
-Section square_bij.
+Section square_bij_def.
 
     Context (n : nat).
 
@@ -18,25 +18,42 @@ Section square_bij.
         fun m : nat =>
             ((m / n), (m mod n)).
 
+End square_bij_def.
+
+Section square_bij_prop.
+
+    Context (n : nat).
+
     Lemma is_bij_square :
-        ∀ c : nat * nat, square_bij_inv (square_bij c) = c.
+        ∀ c : nat * nat, square_bij_inv n (square_bij n c) = c.
     Admitted.
 
     Lemma is_bij_square_inv :
-        ∀ m : nat, square_bij (square_bij_inv m) = m.
+        ∀ m : nat, square_bij n (square_bij_inv n m) = m.
+    Admitted.
+
+    Lemma square_bij_corner :
+        ∀ n' : nat,
+            square_bij (S n) (n', n) = ((S n') * (S n) - 1).
+    Admitted.
+
+    Lemma square_bij_inv_corner :
+        ∀ n' : nat,
+            square_bij_inv (S n) ((S n') * (S n) - 1) = (n', n).
     Admitted.
 
     Lemma confined_square_inv : ∀ n' : nat,
-        ∀ m : nat, m < n * n' ->
-            let (k1, k2) := square_bij_inv m in
-            k1 < n ∧ k2 < n'.
+        ∀ m : nat, m <= S n' * S n - 1 ->
+            let (k1, k2) := square_bij_inv (S n) m in
+            k1 <= n' ∧ k2 <= n.
     Admitted.
-
-    Open Scope nat_scope.
 
     Lemma confined_square : ∀ n' : nat,
         ∀ k1 k2 : nat,
-            k1 < n ∧ k2 < n' -> square_bij (k1, k2) < (n * n').
+            k1 <= n' ∧ k2 <= n -> square_bij (S n) (k1, k2) <= (S n' * S n) - 1.
     Admitted.
 
-End square_bij.
+End square_bij_prop.
+
+Global Opaque square_bij.
+Global Opaque square_bij_inv.
